lean/test/bpf/symeval_harness.lean
@@ -32,18 +32,18 @@ meta def bpf_path : string := (by tactic.io.from_env_var "BPF_BIN_PATH" "test/bp
 def progbits : list bool :=
 (by tactic.io.from_le_quadword_file_as_be_bits bpf_path)
 
-def proof : sat.proof.default.proof :=
-by semidecision.by_oracle (bpf.decision.default.binary_safety_via_reduce_to_smt_oracle fuel) (default _, progbits)
+-- def proof : sat.proof.default.proof :=
+-- by semidecision.by_oracle (bpf.decision.default.binary_safety_via_reduce_to_smt_oracle fuel) (default _, progbits)
 
-theorem binary_program_safety : bpf.binary_safe progbits :=
-bpf.safe_of_erased_regs $
-λ regs, semidec_trivial (bpf.decision.default.decide_binary_safety_via_reduce_to_smt fuel (regs, progbits) proof)
+-- theorem binary_program_safety : bpf.binary_safe progbits :=
+-- bpf.safe_of_erased_regs $
+-- λ regs, semidec_trivial (bpf.decision.default.decide_binary_safety_via_reduce_to_smt fuel (regs, progbits) proof)
 
-def program : bpf.cfg.trie_program :=
-(by tactic.io.exact_io $ tactic.io.read_le_quadword_file_as_bpf_program bpf_path)
+-- def program : bpf.cfg.trie_program :=
+-- (by tactic.io.exact_io $ tactic.io.read_le_quadword_file_as_bpf_program bpf_path)
 
-theorem program_safety : bpf.cfg.safe program :=
-bpf.trie_safe_of_erased_regs $
-λ regs, semidec_trivial (bpf.decision.default.decide_safe_with_regs_via_reduce_to_smt fuel (program, regs) proof)
+-- theorem program_safety : bpf.cfg.safe program :=
+-- bpf.trie_safe_of_erased_regs $
+-- λ regs, semidec_trivial (bpf.decision.default.decide_safe_with_regs_via_reduce_to_smt fuel (program, regs) proof)
 
 end test_bpf
